finished overhaul and refactoring

theories/CADP.v
@@ -5,6 +5,20 @@ Require Import PeanoNat.
 Require Import Notations.
 Require Export Bool.
 
+Notation "x :: l" := (cons x l) (at level 60, right associativity).
+Notation "[ ]" := nil.
+Notation "[ x ; .. ; y ]" := (cons x .. (cons y nil) ..).
+
+Fixpoint app {X:Type} (l1 l2 : list X) : list X :=
+match l1 with
+| nil    => l2
+| h :: t => h :: (app t l2)
+end.
+
+
+(*************************************************************************)
+(**** Basic defs *********************************************************)
+(*************************************************************************)
 
 Definition index : Type := option nat.
 Definition pid   : Type := nat.
@@ -18,31 +32,74 @@ Definition Nil   : index := None.
 (* we dont need new_i, only i and j *)
 Definition lock : Type := index * index.
 
+Module Lock.
+  Definition initial : lock := (None, None).
+End Lock.
+
+
 Module Index.
 
-  Definition Initial : index := Nil.
+  Definition initial : index := Nil.
 
   Definition of_pid (i : pid) : index := Some i.
 
+  Definition to_nat (i : index) : nat :=
+    match i with
+    | None => 0
+    | Some n => n
+    end.
+
+  Definition is_nil (i : index) : bool :=
+    match i with
+    | None => false
+    | _ => true
+    end.
+
+  Definition eqb (i:index) (j:index) : bool :=
+    match i, j with
+    | None, None => true
+    | Some n, Some m => Nat.eqb n m
+    | _, _ => false
+    end.
+
+  Definition is_index (n:option nat) : bool := true.
 
 End Index.
+
+
+Module PID.
+
+  Definition is_pid (n : nat) : bool := if Nat.eqb n 0 then false else true.
+
+  Definition to_nat (p:pid) : nat := p.
+
+End PID.
 
 
 
 Module IBool.
 
   Definition of_index (i:index) : option bool :=
-  match i with
-  | None => None
-  | Some n =>
-    match n with
-    | 0 => Some false
-    | 1 => Some true
-    | _ => None
-    end
-  end.
+    match i with
+    | None => None
+    | Some n =>
+      match n with
+      | 0 => Some false
+      | 1 => Some true
+      | _ => None
+      end
+    end.
 
   Definition of_bool (b:bool) : ibool := if b then 1 else 0.
+
+  Definition to_nat (b:ibool) : nat := b.
+
+  Definition is_ibool (n:nat) : bool :=
+    match n with
+    | 0 => true
+    | 1 => true
+    | _ => false
+    end.
 
   Definition is_some (b:option ibool) : bool :=
     match b with
@@ -55,8 +112,10 @@ End IBool.
 
 
 
+(*************************************************************************)
+(**** Memory *************************************************************)
+(*************************************************************************)
 Module Memory.
-
 
   (**********************************)
   (**** Qnode ***********************)
@@ -67,44 +126,29 @@ Module Memory.
     ; locked : ibool }.
 
   Module Qnode.
-
     Definition initial : qnode := Build_qnode None 0.
 
-    (* redundant ? *)
     Module _Get.
-
       Definition next   (q:qnode) : index := (next q).
       Definition locked (q:qnode) : ibool := (locked q).
-
     End _Get.
 
 
     Module _Set.
-
-      Definition next   (i:index) (q:qnode) : qnode := Build_qnode i (_Get.locked q).
-      Definition locked (b:ibool) (q:qnode) : qnode := Build_qnode (_Get.next q) b.
-
+      Definition next   (i:index) (q:qnode) : qnode :=
+        Build_qnode i (Qnode._Get.locked q).
+      Definition locked (b:ibool) (q:qnode) : qnode :=
+        Build_qnode (Qnode._Get.next q) b.
     End _Set.
-
 
   End Qnode.
 
 
   (**********************************)
-  (**** mem Type, notation & app ****)
+  (**** mem Type & app **************)
   (**********************************)
 
   Definition mem : Type := list qnode.
-
-  Notation "x :: l" := (cons x l) (at level 60, right associativity).
-  Notation "[ ]" := nil.
-  Notation "[ x ; .. ; y ]" := (cons x .. (cons y nil) ..).
-
-  Fixpoint app (l1 l2 : mem) : mem :=
-    match l1 with
-    | nil    => l2
-    | h :: t => h :: (app t l2)
-    end.
 
   (**********************************)
   (**** Creating & Initializing *****)
@@ -219,12 +263,12 @@ Module Memory.
       end.
 
   End _Set.
-
-
 End Memory.
 
 
-
+(*************************************************************************)
+(**** Vars ***************************************************************)
+(*************************************************************************)
 Module Vars.
 
   Record vars :=
@@ -233,23 +277,21 @@ Module Vars.
   ; var_next        : index        (* release *)
   ; var_swap        : option ibool (* release *) }.
 
+  Definition initial : vars := Build_vars None None None None.
+
   Inductive var : Type :=
     | PREDECESSOR
     | LOCKED
     | NEXT
     | SWAP
-    (* | PID *)
+    | PID
     (* | NIL *)
     .
 
-  Inductive val : Type :=
-  | INDEX : index        -> val (* not yet used *)
-  | IBOOL : option ibool -> val (* not yet used *)
-  | VAR : var -> val
-  | TRU : val
-  | FLS : val
-  | NIL : val
-  .
+
+  Module Kind.
+    Inductive kind : Type := | INDEX | IBOOL | PID.
+  End Kind.
 
 
   Module _Get.
@@ -284,242 +326,365 @@ Module Vars.
 End Vars.
 
 
+(*************************************************************************)
+(**** Value **************************************************************)
+(*************************************************************************)
+Module Val.
+  Inductive val : Type :=
+  | INDEX : index        -> val
+  | IBOOL : option ibool -> val
+  | PID : val
+  | VAR : Vars.var -> val
+  | TRU : val
+  | FLS : val
+  | NIL : val
+  .
+End Val.
 
+
+(*************************************************************************)
+(**** (Global) Resource **************************************************)
+(*************************************************************************)
+Module Resource.
+  Definition resource : Type := Memory.mem * lock.
+  Definition initial (n:nat) : resource := (Memory.initial n, Lock.initial).
+
+  Module _Get.
+    Definition mem (s:resource) : Memory.mem :=
+      match s with
+      | (mem, lock) => mem
+      end.
+
+    Definition lock (s:resource) : lock :=
+      match s with
+      | (mem, lock) => lock
+      end.
+
+    Module Lock.
+      Definition i (s:resource) : index :=
+        match (lock s) with
+        | (i, j) => i
+        end.
+
+      Definition j (s:resource) : index :=
+        match (lock s) with
+        | (i, j) => j
+        end.
+
+    End Lock.
+  End _Get.
+
+
+  Module _Set.
+    Module Lock.
+      Definition i (new_i:index) (s:resource) : resource :=
+        match (_Get.lock s) with
+        | (i, j) => (_Get.mem s, (new_i, j))
+        end.
+
+      Definition j (new_j:index) (s:resource) : resource :=
+        match (_Get.lock s) with
+        | (i, j) => (_Get.mem s, (i, new_j))
+        end.
+
+    End Lock.
+  End _Set.
+End Resource.
+
+
+(*************************************************************************)
+(**** (Local) State ******************************************************)
+(*************************************************************************)
 Module State.
 
   Definition local : Type := pid * Vars.vars.
 
-  Definition resource : Type := Memory.mem * lock.
+  Definition create (p:pid) : local := (p, Vars.initial).
 
-  Definition global : Type := (list local) * resource.
+  Module _Get.
+    Definition pid (s:local) : pid :=
+      match s with
+      | (pid, vars) => pid
+      end.
+
+    Definition vars (s:local) : Vars.vars :=
+      match s with
+      | (pid, vars) => vars
+      end.
 
 
-  Module _Local.
+    Module Var.
+      Definition predecessor (s:local) : index :=
+        Vars._Get.predecessor (vars s).
+      Definition locked (s:local) : option ibool := Vars._Get.locked (vars s).
+      Definition next (s:local) : index := Vars._Get.next (vars s).
+      Definition swap (s:local) : option ibool := Vars._Get.swap (vars s).
 
-    Module _Get.
+    End Var.
 
-      Definition pid (s:local) : pid :=
+    Definition var (v:Vars.var) (s:local) : option nat :=
+      match v with
+      | Vars.PREDECESSOR => Var.predecessor s
+      | Vars.LOCKED      => Var.locked s
+      | Vars.NEXT        => Var.next s
+      | Vars.SWAP        => Var.swap s
+      | Vars.PID         => Some (pid s)
+      end.
+
+    Definition val (v:Val.val) (s:local) : option nat :=
+      match v with
+      | Val.INDEX i => i
+      | Val.IBOOL b => b
+      | Val.PID     => Some (pid s)
+      | Val.VAR v   => var v s
+      | Val.TRU     => Some 1
+      | Val.FLS     => Some 0
+      | Val.NIL     => Nil
+      end.
+
+  End _Get.
+
+
+  Module _Set.
+    Module Var.
+
+      Definition predecessor (i:index) (s:local) : local :=
         match s with
-        | (pid, vars) => pid
+        | (pid, vars) => (pid, Vars._Set.predecessor i vars)
         end.
 
-      Definition vars (s:local) : Vars.vars :=
-        match s with
-        | (pid, vars) => vars
-        end.
-
-
-      Module Var.
-
-        Definition predecessor (s:local) : index := Vars._Get.predecessor (vars s).
-
-        Definition locked (s:local) : option ibool := Vars._Get.locked (vars s).
-
-        Definition next (s:local) : index := Vars._Get.next (vars s).
-
-        Definition swap (s:local) : option ibool := Vars._Get.swap (vars s).
-
-      End Var.
-
-      Definition var (v:Vars.var) (s:local) : option nat :=
-        match v with
-        | Vars.PREDECESSOR => Var.predecessor s
-        | Vars.LOCKED      => Var.locked s
-        | Vars.NEXT        => Var.next s
-        | Vars.SWAP        => Var.swap s
-        (* | PID         => Some (pid s) *)
-        (* | NIL         => None *)
-        end.
-
-      Definition val (v:Vars.val) (s:local) : option nat :=
-        match v with
-        | Vars.INDEX i => i
-        | Vars.IBOOL b => b
-        | Vars.VAR v   => var v s
-        | Vars.TRU     => Some 1
-        | Vars.FLS     => Some 0
-        | Vars.NIL     => Nil
-        end.
-
-    End _Get.
-
-
-    Module _Set.
-
-
-      Module Var.
-
-        Definition predecessor (i:index) (s:local) : local :=
-          match s with
-          | (pid, vars) => (pid, Vars._Set.predecessor i vars)
-          end.
-
-        Definition locked (b:ibool) (s:local) : local :=
+      Definition locked (b:ibool) (s:local) : local :=
         match s with
         | (pid, vars) => (pid, Vars._Set.locked b vars)
         end.
 
-        Definition next (i:index) (s:local) : local :=
-          match s with
-          | (pid, vars) => (pid, Vars._Set.next i vars)
-          end.
+      Definition next (i:index) (s:local) : local :=
+        match s with
+        | (pid, vars) => (pid, Vars._Set.next i vars)
+        end.
 
-        Definition swap (b:ibool) (s:local) : local :=
+      Definition swap (b:ibool) (s:local) : local :=
         match s with
         | (pid, vars) => (pid, Vars._Set.swap b vars)
         end.
 
-      End Var.
-
-    End _Set.
-
-  End _Local.
-
-
-  Module _Resource.
-
-
-    Module _Get.
-
-      Definition mem (s:resource) : Memory.mem :=
-        match s with
-        | (mem, lock) => mem
-        end.
-
-      Definition lock (s:resource) : lock :=
-        match s with
-        | (mem, lock) => lock
-        end.
-
-
-      Module Lock.
-
-        Definition i (s:resource) : index :=
-          match (lock s) with
-          | (i, j) => i
-          end.
-
-        Definition j (s:resource) : index :=
-          match (lock s) with
-          | (i, j) => j
-          end.
-
-      End Lock.
-
-    End _Get.
-
-
-    Module _Set.
-
-
-      Module Lock.
-
-        Definition i (new_i:index) (s:resource) : resource :=
-          match (_Get.lock s) with
-          | (i, j) => (_Get.mem s, (new_i, j))
-          end.
-
-        Definition j (new_j:index) (s:resource) : resource :=
-          match (_Get.lock s) with
-          | (i, j) => (_Get.mem s, (i, new_j))
-          end.
-
-      End Lock.
-
-    End _Set.
-
-  End _Resource.
-
-
-  Module _Global.
-
-
-    Module _Get.
-
-      Definition mem (s:global) : Memory.mem :=
-        match s with
-        | (pids, resource) =>
-          match resource with
-          | (mem, lock) => mem
-          end
-        end.
-
-      Definition lock (s:global) : lock :=
-        match s with
-        | (pids, resource) =>
-          match resource with
-          | (mem, lock) => lock
-          end
-        end.
-
-      End _Get.
-
-  End _Global.
-
-  Inductive state : Type :=
-  | LOCAL  : local  -> state
-  | GLOBAL : global -> state
-  .
-
+    End Var.
+  End _Set.
 End State.
 
 
+(*************************************************************************)
+(**** Environment (local) ************************************************)
+(*************************************************************************)
+Definition env : Type := State.local * Resource.resource.
+
+Module Env.
+  Module _Get.
+
+    Definition local (e:env) : State.local :=
+      match e with | (l, r) => l end.
+
+    Definition pid (e:env) : pid := State._Get.pid (local e).
+    Definition vars (e:env) : Vars.vars := State._Get.vars (local e).
+
+    Module Var.
+      Definition predecessor (e:env) : index :=
+        Vars._Get.predecessor (vars e).
+      Definition locked (e:env) : option ibool :=
+        Vars._Get.locked (vars e).
+      Definition next (e:env) : index :=
+        Vars._Get.next (vars e).
+      Definition swap (e:env) : option ibool :=
+        Vars._Get.swap (vars e).
+
+    End Var.
+
+    Definition var (v:Vars.var) (e:env) : option nat :=
+      State._Get.var v (local e).
+
+    Definition val (v:Val.val) (e:env) : option nat :=
+      State._Get.val v (local e).
+
+    Definition resource (e:env) : Resource.resource :=
+      match e with | (l, r) => r end.
+
+    Definition mem (e:env) : Memory.mem :=
+      Resource._Get.mem (resource e).
+
+    Module Mem.
+      Definition locked_of (i:index) (e:env) : option ibool :=
+        Memory._Get.locked_of i (Env._Get.mem e).
+
+      Definition next_of (i:index) (e:env) : index :=
+        Memory._Get.next_of i (Env._Get.mem e).
+
+    End Mem.
+
+
+    Definition lock (e:env) : lock :=
+      Resource._Get.lock (resource e).
+
+    Module Lock.
+      Definition i (e:env) : index :=
+        Resource._Get.Lock.i (Env._Get.resource e).
+      Definition j (e:env) : index :=
+        Resource._Get.Lock.j (Env._Get.resource e).
+
+    End Lock.
+  End _Get.
+
+
+  Module _Set.
+    Module Var.
+
+      Definition predecessor (i:index) (e:env) : env :=
+        match e with
+        | (l, r) => ((State._Set.Var.predecessor i l), r)
+        end.
+
+      Definition locked (b:ibool) (e:env) : env :=
+        match e with
+        | (l, r) => ((State._Set.Var.locked b l), r)
+        end.
+
+      Definition next (i:index) (e:env) : env :=
+        match e with
+        | (l, r) => ((State._Set.Var.next i l), r)
+        end.
+
+      Definition swap (b:ibool) (e:env) : env :=
+        match e with
+        | (l, r) => ((State._Set.Var.swap b l), r)
+        end.
+
+    End Var.
+
+    Definition resource (r:Resource.resource) (e:env) : env :=
+      (Env._Get.local e, r).
+
+    Definition mem (m:Memory.mem) (e:env) : env :=
+      (Env._Get.local e, (m, Env._Get.lock e)).
+
+    Module Mem.
+      Definition locked_of (i:index) (b:ibool) (e:env) : option env :=
+        match (Memory._Set.locked_of i b (Env._Get.mem e)) with
+        | None => None
+        | Some m => Some (mem m e)
+        end.
+
+      Definition next_of (i:index) (n:index) (e:env) : option env :=
+        match (Memory._Set.next_of i n (Env._Get.mem e)) with
+        | None => None
+        | Some m => Some (mem m e)
+        end.
+
+    End Mem.
+
+    Definition lock (l:lock) (e:env) : env :=
+      (Env._Get.local e, (Env._Get.mem e, l)).
+
+    Module Lock.
+      Definition i (new_i:index) (e:env) : env :=
+        resource (Resource._Set.Lock.i new_i (Env._Get.resource e)) e.
+
+      Definition j (new_j:index) (e:env) : env :=
+        resource (Resource._Set.Lock.j new_j (Env._Get.resource e)) e.
+
+    End Lock.
+
+  End _Set.
+
+
+  Module Handle.
+
+    (** [read_next e] will set var [next] to be the value
+        currently of the [qnode.next] corresponding to the
+        [pid] of the process in the state. *)
+    Definition read_next (e:env) : env :=
+      let p : pid        := Env._Get.pid e in
+      let new_next:index := Env._Get.Mem.next_of (Index.of_pid p) e in
+      Env._Set.Var.next new_next e.
+
+    (** [read_locked e] will set var [locked] to be
+        the value of the [qnode.locked] corresponding
+        to the [pid] of the process in the state.
+        ! ! ! it requires that [qnode.locked] is not None. *)
+    Definition read_locked (e:env) : env :=
+    let p : pid        := Env._Get.pid e in
+    match (Env._Get.Mem.locked_of (Index.of_pid p) e) with
+    | None => e (* shouldn't happen, semantics guard from this. *)
+    | Some new_locked => Env._Set.Var.locked new_locked e
+    end.
+
+    (*  *)
+    Definition write_next (to_write:Vars.var) (next:Val.val) (e:env) : env :=
+      match (Env._Get.val next e) with
+      | None => e (* shouldn't happen, semantics guard from this. *)
+      | Some next' =>
+        let next' : index := Index.of_pid next' in
+        match (Env._Get.var to_write e) with
+        | None => e (* shouldn't happen, semantics guard from this. *)
+        | Some to_write' =>
+          match (Env._Set.Mem.next_of (Index.of_pid to_write') next' e) with
+          | None => e (* shouldn't happen, semantics guard from this. *)
+          | Some e' => e'
+          end
+        end
+      end.
+
+    (*  *)
+    Definition write_locked (to_write:Vars.var) (locked:Val.val) (e:env) : env :=
+      match (Env._Get.val locked e) with
+        | None => e (* shouldn't happen, semantics guard from this. *)
+        | Some locked' =>
+        match (IBool.is_ibool locked') with
+        | false => e (* shouldn't happen, semantics guard from this. *)
+        | true =>
+          match (Env._Get.var to_write e) with
+          | None => e (* shouldn't happen, semantics guard from this. *)
+          | Some to_write' =>
+            let to_write' : index := Index.of_pid to_write' in
+            match (Env._Set.Mem.locked_of to_write' locked' e) with
+            | None => e (* shouldn't happen, semantics guard from this. *)
+            | Some e' => e'
+            end
+          end
+        end
+      end.
+
+    (*  *)
+    Definition fetch_and_store (e:env) : env :=
+      (* store [Lock.i] in [Vars.predecessor]. *)
+      let i : index := Env._Get.Lock.i e in
+      let e' : env := Env._Set.Var.predecessor i e in
+      (* set [Lock.i] to [pid]. *)
+      let p : pid := Env._Get.pid e' in
+      Env._Set.Lock.i (Index.of_pid p) e'.
+
+    (*  *)
+    Definition compare_and_swap (e:env) : env :=
+      let i : index := Env._Get.Lock.i e in
+      let j : index := Env._Get.Lock.j e in
+      (* set [Lock.j] to [pid]. *)
+      let p : pid := Env._Get.pid e in
+      let e' : env := Env._Set.Lock.j (Index.of_pid p) e in
+      let are_eq : bool := Index.eqb i j in
+      Env._Set.Var.swap
+        (IBool.of_bool are_eq)
+        (* also, if eq then reset [i] to Nil. *)
+        (if are_eq then Env._Set.Lock.i Nil e' else e').
+
+    End Handle.
+
+End Env.
+
+
+
+(*************************************************************************)
+(**** Process ************************************************************)
+(*************************************************************************)
 Module Process.
 
-  Definition env : Type := State.local * State.resource.
-
-  Module Env.
-
-    Module _Get.
-
-      Definition local (e:env) : State.local :=
-        match e with
-        | (l, r) => l
-        end.
-
-      Definition pid (e:env) : pid := State._Local._Get.pid (local e).
-      Definition vars (e:env) : Vars.vars := State._Local._Get.vars (local e).
-
-      Definition resource (e:env) : State.resource :=
-        match e with
-        | (l, r) => r
-        end.
-
-      Definition mem (e:env) : Memory.mem := State._Resource._Get.mem (resource e).
-      Definition lock (e:env) : lock := State._Resource._Get.lock (resource e).
-
-    End _Get.
-
-
-    Module _Set.
-
-      Module Var.
-
-        Definition predecessor (i:index) (e:env) : env :=
-          match e with
-          | (l, r) => ((State._Local._Set.Var.predecessor i l), r)
-          end.
-
-        Definition locked (b:ibool) (e:env) : env :=
-          match e with
-          | (l, r) => ((State._Local._Set.Var.locked b l), r)
-          end.
-
-        Definition next (i:index) (e:env) : env :=
-          match e with
-          | (l, r) => ((State._Local._Set.Var.next i l), r)
-          end.
-
-        Definition swap (b:ibool) (e:env) : env :=
-          match e with
-          | (l, r) => ((State._Local._Set.Var.swap b l), r)
-          end.
-
-      End Var.
-
-    End _Set.
-
-  End Env.
 
 
   Module Expr.
@@ -528,14 +693,14 @@ Module Process.
       | NOT : expr -> expr
       | VAR : Vars.var -> expr
       | NAT : nat -> expr
-      | IBOOL : nat -> expr
-      | EQ  : nat -> nat -> expr
+      | IBOOL : ibool -> expr
+      | INDEX : index -> expr
+      | CAST : expr -> Vars.Kind.kind -> expr
+      | PID : pid -> expr
+      | EQ  : expr -> expr -> expr
       | TT  : expr
       | FF  : expr
-      .
-
-    Inductive ibool_guard : option ibool -> Prop :=
-      | SOME_IBOOL : forall (b:ibool), ibool_guard (Some b)
+      | NIL : expr
       .
 
     Inductive eval : (expr * env) -> (expr * env) -> Prop :=
@@ -546,10 +711,94 @@ Module Process.
       | NOT_TT : forall e, eval (NOT TT, e) (FF, e)
       | NOT_FF : forall e, eval (NOT FF, e) (TT, e)
 
-      | EQ_NAT : forall n e,
-        eval (EQ n n) (TT)
+      | VAR_PREDECESSOR : forall v e,
+        (Env._Get.Var.predecessor e)=v ->
+        eval (VAR Vars.PREDECESSOR, e) (INDEX v, e)
 
+      | VAR_LOCKED : forall v b e,
+        (Env._Get.Var.locked e)=v /\ v=(Some b) ->
+        eval (VAR Vars.LOCKED, e) (IBOOL b, e)
+
+      | VAR_NEXT : forall v e,
+        (Env._Get.Var.next e)=v ->
+        eval (VAR Vars.NEXT, e) (INDEX v, e)
+
+      | VAR_SWAP : forall v b e,
+        (Env._Get.Var.swap e)=v /\ v=(Some b) ->
+        eval (VAR Vars.SWAP, e) (IBOOL b, e)
+
+      | CAST_PID_TO_INDEX : forall p e,
+        eval (CAST (PID p) Vars.Kind.INDEX, e) (INDEX (Index.of_pid p), e)
+
+      | CAST_INDEX_TO_PID : forall i n e,
+        (i=Some(S n)) ->
+        eval (CAST (INDEX i) Vars.Kind.PID, e) (PID n, e)
+
+      | EQ_TT_NAT : forall n m e,
+        (Nat.eqb n m)=true ->
+        eval (EQ (NAT n) (NAT m), e) (TT, e)
+
+      | EQ_FF_NAT : forall n m e,
+        (Nat.eqb n m)=false ->
+        eval (EQ (NAT n) (NAT m), e) (FF, e)
+
+      | EQ_TT_IBOOL : forall n m e,
+        ((IBool.is_ibool n)=true /\ (IBool.is_ibool m)=true)
+        /\ (Nat.eqb (IBool.to_nat n) (IBool.to_nat m))=true ->
+        eval (EQ (IBOOL n) (IBOOL m), e) (TT, e)
+
+      | EQ_FF_IBOOL : forall n m e,
+        ((IBool.is_ibool n)=false \/ (IBool.is_ibool m)=false)
+        \/ (Nat.eqb (IBool.to_nat n) (IBool.to_nat m))=false ->
+        eval (EQ (IBOOL n) (IBOOL m), e) (FF, e)
+
+      | EQ_TT_INDEX : forall n m e,
+        (Nat.eqb (Index.to_nat n) (Index.to_nat m))=true ->
+        eval (EQ (INDEX n) (INDEX m), e) (TT, e)
+
+      | EQ_FF_INDEX : forall n m e,
+        (Nat.eqb (Index.to_nat n) (Index.to_nat m))=false ->
+        eval (EQ (INDEX n) (INDEX m), e) (TT, e)
+
+      | EQ_TT_PID : forall n m e,
+        ((PID.is_pid n)=true /\ (PID.is_pid m)=true)
+        /\ (Nat.eqb (PID.to_nat n) (PID.to_nat m))=true ->
+        eval (EQ (PID n) (PID m), e) (TT, e)
+
+      | EQ_FF_PID : forall n m e,
+        ((PID.is_pid n)=false \/ (PID.is_pid m)=false)
+        \/ (Nat.eqb (PID.to_nat n) (PID.to_nat m))=false ->
+        eval (EQ (PID n) (PID m), e) (TT, e)
+
+      | EQ_TT_NIL_NIL : forall e,
+        eval (EQ NIL NIL, e) (TT, e)
+
+      | EQ_TT_NIL_INDEX_L : forall n e,
+        (Index.is_nil n)=true ->
+        eval (EQ (INDEX n) NIL, e) (TT, e)
+
+      | EQ_FF_NIL_INDEX_L : forall n e,
+        (Index.is_nil n)=false ->
+        eval (EQ (INDEX n) NIL, e) (FF, e)
+
+      | EQ_TT_NIL_INDEX_R : forall n e,
+        (Index.is_nil n)=true ->
+        eval (EQ NIL (INDEX n), e) (TT, e)
+
+      | EQ_FF_NIL_INDEX_R : forall n e,
+        (Index.is_nil n)=false ->
+        eval (EQ NIL (INDEX n), e) (FF, e)
+
+      | EQ_FF_NIL_PID_L : forall n e,
+        (PID.is_pid n)=true ->
+        eval (EQ (PID n) NIL, e) (FF, e)
+
+      | EQ_FF_NIL_PID_R : forall n e,
+        (PID.is_pid n)=true ->
+        eval (EQ NIL (PID n), e) (FF, e)
       .
+
+    Print eval.
 
   End Expr.
 
@@ -565,111 +814,93 @@ Module Process.
       | READ_NEXT   : act
       | READ_LOCKED : act
 
-      | WRITE_NEXT   : Vars.var -> Vars.val -> act
-      | WRITE_LOCKED : Vars.var -> Vars.val -> act
+      | WRITE_NEXT   : Vars.var -> Val.val -> act
+      | WRITE_LOCKED : Vars.var -> Val.val -> act
 
       | FETCH_AND_STORE  : act
       | COMPARE_AND_SWAP : act
       .
 
-      Module Handle.
+    Inductive guard : (act * env) -> Prop :=
 
-        (** [read_next e] will set var [next] to be the value
-            currently of the [qnode.next] corresponding to the
-            [pid] of the process in the state. *)
-        Definition read_next (e:env) : env :=
-          let m : Memory.mem := Env._Get.mem e in
-          let p : pid        := Env._Get.pid e in
-          let new_next:index := Memory._Get.next_of (Index.of_pid p) m in
-          Env._Set.Var.next new_next e.
+      (* no guard. *)
+      | G_READ_NEXT : forall e,
+        guard (READ_NEXT, e)
 
-        (** [read_locked e] will set var [locked] to be
-            the value of the [qnode.locked] corresponding
-            to the [pid] of the process in the state.
-            ! ! ! it requires that [qnode.locked] is not None. *)
-        Definition read_locked (e:env) : env :=
-        let m : Memory.mem := Env._Get.mem e in
-        let p : pid        := Env._Get.pid e in
-        match (Memory._Get.locked_of (Index.of_pid p) m) with
-        | None => e (* should not happen, semantics guard this from happening *)
-        | Some new_locked =>
-          Env._Set.Var.locked new_locked e
-        end.
+      (* check that [qnode.next] of [pid] is not None. *)
+      | G_READ_LOCKED : forall v b e,
+        (Memory._Get.next_of
+          (Index.of_pid (Env._Get.pid e))
+          (Env._Get.mem e))=v /\ v=(Some b) ->
+        guard (READ_LOCKED, e)
 
+      (* check that [vqi] is not None. *)
+      | G_WRITE_NEXT : forall vqi qi vni ni e,
+        (Env._Get.var vqi e)=(Some qi) /\ (PID.is_pid qi)=true /\
+        (Env._Get.val vni e)=(Some ni) /\ (PID.is_pid ni)=true /\
+        vni=(Val.INDEX (Some ni)) ->
+        guard (WRITE_NEXT vqi vni, e)
 
-      End Handle.
+      (* check [vqi] and [vnl] are not None, and that [vnl] is Some ibool. *)
+      | G_WRITE_LOCKED : forall vqi qi vnl nl e,
+        (Env._Get.var vqi e)=(Some qi) /\ (PID.is_pid qi)=true     /\
+        (Env._Get.val vnl e)=(Some nl) /\ (IBool.is_ibool nl)=true /\
+        vnl=(Val.IBOOL (Some nl)) ->
+        guard (WRITE_LOCKED vqi vnl, e)
 
-      Inductive guard : (act * env) -> Prop :=
+      (* no guard. *)
+      | G_FETCH_AND_STORE : forall e,
+        guard (FETCH_AND_STORE, e)
 
-        | G_READ_NEXT : forall (e:env),
-          guard (READ_NEXT, e)
+      (* no guard. *)
+      | G_COMPARE_AND_SWAP : forall e,
+        guard (COMPARE_AND_SWAP, e)
+      .
 
-        | G_READ_LOCKED : forall (e:env) (p:pid) (m:Memory.mem) (l:ibool),
-          Expr.ibool_guard (Memory._Get.next_of (Index.of_pid p) m) ->
-          guard (READ_LOCKED, e)
+    Print guard.
 
-        | G_WRITE_NEXT : forall vr vl (e:env),
-          guard (WRITE_NEXT vr vl, e)
+    Definition update_env (a:act) (e:env) : env :=
+      match a with
+      (* CS Access *)
+      | NCS   => e
+      | ENTER => e
+      | LEAVE => e
 
-        | G_WRITE_LOCKED : forall vr vl (e:env) (p:pid) (m:Memory.mem) (l:ibool),
-          guard (WRITE_LOCKED vr vl, e)
+      (* Memory Access *)
+      | READ_NEXT    => Env.Handle.read_next e
+      | READ_LOCKED  => Env.Handle.read_locked e
 
-        .
+      | WRITE_NEXT to_write next =>
+          Env.Handle.write_next to_write next e
 
-      Definition update_env (a:act) (e:env) : env :=
-        match a with
-        (* CS Access *)
-        | NCS   => e
-        | ENTER => e
-        | LEAVE => e
+      | WRITE_LOCKED to_write locked =>
+          Env.Handle.write_locked to_write locked e
 
-        (* Memory Access *)
-        | READ_NEXT    => Handle.read_next e
-        | READ_LOCKED  => Handle.read_locked e
-        (* bind_locked (get_mem_qnode_locked (Index (get_pid s)) s) s *)
+      (* Lock Access *)
+      | FETCH_AND_STORE  => Env.Handle.fetch_and_store e
+      | COMPARE_AND_SWAP => Env.Handle.compare_and_swap e
 
-        | WRITE_NEXT   pid_to_write next_pid  => e
-                          (* set_mem_qnode_next   (get_var pid_to_write s) (get_val next_pid  s) s *)
-
-        | WRITE_LOCKED pid_to_write is_locked => e
-                          (* set_mem_qnode_locked (get_var pid_to_write s) (get_val is_locked s) s *)
-
-        (* Lock Access *)
-        | FETCH_AND_STORE  => e
-        (* set_lock_i (Index (get_pid s)) (bind_predecessor (get_lock_i s) s) *)
-        | COMPARE_AND_SWAP => e
-        (* let s1 := set_lock_j (Index (get_pid s)) s in
-                              let s2 := bind_swap (index_eq (get_lock_i s1) (get_lock_j s1)) s1 in
-                              let s3 := set_lock_i 0 s2 in s3 *)
-        end.
+      end.
 
   End Operation.
 
   Inductive tm : Type :=
-    | TYPE_ERR : tm
-    | OK    : tm                      (* no-op *)
+    | ERR : tm (* error *)
+    | OK  : tm (* no-op *)
+    | END : tm (* termination *)
+
+    | IF  : Expr.expr -> tm -> tm -> tm
 
     | ACT : Operation.act -> tm
 
     | SEQ : tm -> tm -> tm
 
-    | IF    : Expr.expr -> tm -> tm -> tm    (* condition -> if true -> if false -> ... *)
-
-    (* | VAL    : Vars.val  -> tm
-    | NOT    : tm   -> tm
-    | EQ_N   : nat  -> nat -> tm
-    | EQ_B   : bool -> bool -> tm
-    | IS_TRU : tm   -> tm
-    | IS_NIL : tm   -> tm
-
-    | TT   : tm        (* true *)
-    | FF   : tm        (* false *)
- *)
     | LOOP      : tm -> tm (* inner loop body -> *)
     | LOOP_END  : tm
 
-    | LOOP_OVER : iloop -> tm -> tm -> tm (* loop id -> body -> outer continuation -> ... *)
-    | BREAK     : iloop -> tm             (* loop id -> ... *)
+    (* loop id -> body -> outer continuation -> ... *)
+    | LOOP_OVER : iloop -> tm -> tm -> tm
+    | BREAK     : iloop -> tm
     .
 
   (* following: https://softwarefoundations.cis.upenn.edu/plf-current/Types.html *)
@@ -686,26 +917,16 @@ Module Process.
 
   Fixpoint subst (new old:tm) (loops:bool) : tm :=
     match old with
-    | TYPE_ERR => TYPE_ERR
+    | ERR => ERR
     | OK   => OK
+    | END   => END
 
     | IF c t e => IF c (subst new t loops) (subst new e loops)
 
-
-    | VAL t => VAL t
-    | NOT t      => NOT t
-    | EQ_N a b   => EQ_N a b
-    | EQ_B a b   => EQ_B a b
-    | IS_TRU a   => IS_TRU a
-    | IS_NIL t   => IS_NIL t
-    (* | VAR v      => VAR v *)
-
-    | TT => TT
-    | FF => FF
-
     | ACT a => ACT a
 
-    | SEQ l r => SEQ l (subst new r loops) (* do not substitute in other body *)
+    (* do not substitute in other body *)
+    | SEQ l r => SEQ l (subst new r loops)
 
     | LOOP b   => if loops then LOOP (subst new b loops) else LOOP b
     | LOOP_END => new
@@ -714,317 +935,187 @@ Module Process.
     | BREAK l         => BREAK l
     end.
 
-    Module Semantics.
+  Module Semantics.
 
-      Inductive action : Type :=
-      | SILENT : action
-      | LABEL  : Operation.act -> pid -> action.
+    Inductive action : Type :=
+    | SILENT : action
+    | LABEL  : Operation.act -> pid -> action.
 
-      Reserved Notation "t '--<{' a '}>-->' t'" (at level 40).
+    Reserved Notation "t '--<{' a '}>-->' t'" (at level 40).
 
-      Inductive step : (tm * env) -> action -> (tm * env) -> Prop :=
+    Inductive step : (tm * env) -> action -> (tm * env) -> Prop :=
 
-        | ACT : forall a (e:env),
-          (Operation.guard (a, e)) ->
-          (ACT a, e) --<{LABEL a (Env._Get.pid e)}>--> (OK, Operation.update_env a e)
+      | ACT : forall a (e:env),
+        (Operation.guard (a, e)) ->
+        (ACT a, e) --<{LABEL a (Env._Get.pid e)}>--> (OK, Operation.update_env a e)
 
-        | SEQ : forall a l1 l2 r e1 e2,
-          (l1, e1) --<{a}>--> (l2, e2) ->
-          (SEQ l1 r, e1) --<{a}>--> (SEQ l2 r, e2)
+      | SEQ : forall a l1 l2 r e1 e2,
+        (l1, e1) --<{a}>--> (l2, e2) ->
+        (SEQ l1 r, e1) --<{a}>--> (SEQ l2 r, e2)
 
-        | SEQ_END : forall r e,
-          (SEQ OK r, e) --<{SILENT}>--> (r, e)
+      | SEQ_END : forall r e,
+        (SEQ OK r, e) --<{SILENT}>--> (r, e)
 
-        | LOOP  : forall t e,
-          (LOOP t, e) --<{SILENT}>--> (subst t LOOP_END false, e)
+      | LOOP  : forall t e,
+        (LOOP t, e) --<{SILENT}>--> (subst t LOOP_END false, e)
 
-        | BREAK : forall l c e,
-          (LOOP_OVER l (BREAK l) c, e) --<{SILENT}>--> (c, e)
+      | BREAK : forall l c e,
+        (LOOP_OVER l (BREAK l) c, e) --<{SILENT}>--> (c, e)
 
-        | LOOP_OVER : forall a l t1 t2 c e1 e2,
-          (LOOP t1, e1) --<{a}>--> (LOOP t2, e2) ->
-            (LOOP_OVER l t1 c, e1) --<{a}>--> (LOOP_OVER l t2 c, e2)
+      | LOOP_OVER : forall a l t1 t2 c e1 e2,
+        (LOOP t1, e1) --<{a}>--> (LOOP t2, e2) ->
+          (LOOP_OVER l t1 c, e1) --<{a}>--> (LOOP_OVER l t2 c, e2)
 
-        | IF_TT : forall t1 t2 e,
-          (<{ if TT then t1 else t2 }>, e) --<{SILENT}>--> (t1, e)
+      | IF_TT : forall t1 t2 e,
+        (<{ if Expr.TT then t1 else t2 }>, e) --<{SILENT}>--> (t1, e)
 
-        | IF_FF : forall t1 t2 e,
-          (<{ if FF then t1 else t2 }>, e) --<{SILENT}>--> (t2, e)
+      | IF_FF : forall t1 t2 e,
+        (<{ if Expr.FF then t1 else t2 }>, e) --<{SILENT}>--> (t2, e)
 
-        | IF : forall c1 c2 t1 t2 e1,
-          (Expr.eval (c1, e1) (c2, e2)) ->
-          (<{ if c1 then t1 else t2 }>, e1) --<{SILENT}>--> (<{ if c2 then t1 else t2 }>, e2)
+      | IF : forall c1 c2 t1 t2 e,
+        (Expr.eval (c1, e) (c2, e)) ->
+        (<{ if c1 then t1 else t2 }>, e) --<{SILENT}>--> (<{ if c2 then t1 else t2 }>, e)
 
-      where "t '--<{' a '}>-->' t'" := (step t a t').
+    where "t '--<{' a '}>-->' t'" := (step t a t').
 
-
-
-    End Semantics.
+  End Semantics.
 
 End Process.
 
 
+(*************************************************************************)
+(**** System (of processes) **********************************************)
+(*************************************************************************)
+Module System.
+
+  Inductive sys : Type :=
+    | PRC : Process.tm -> State.local -> sys
+    | PAR : sys -> sys -> sys
+    | TERM : sys
+    .
+
+  Module LTS.
+    Reserved Notation "t '--<{' a '}>-->' t'" (at level 40).
+    Reserved Notation "t '==<{' a '}>==>' t'" (at level 40).
+
+    Inductive lts : sys * Resource.resource -> Process.Semantics.action -> sys * Resource.resource -> Prop :=
+
+    (* wrapper for sharing global resource with local process. *)
+      | PRC : forall a t1 t2 s1 s2 r1 r2,
+        (t1, (s1, r1)) --<{a}>--> (t2, (s2, r2)) ->
+        (PRC t1 s1, r1) ==<{a}>==> (PRC t2 s2, r2)
+
+      | PAR_L : forall a l1 l2 r gr1 gr2,
+        (l1, gr1) ==<{a}>==> (l2, gr2) ->
+        (PAR l1 r, gr1) ==<{a}>==> (PAR l2 r, gr2)
+
+      | PAR_R : forall a l r1 r2 gr1 gr2,
+        (r1, gr1) ==<{a}>==> (r2, gr2) ->
+        (PAR l r1, gr1) ==<{a}>==> (PAR l r2, gr2)
+
+      | END_L : forall a ls r gr,
+        (PAR (PRC Process.END ls) r, gr) ==<{a}>==> (r, gr)
+
+      | END_R : forall a l rs gr,
+        (PAR l (PRC Process.END rs), gr) ==<{a}>==> (l, gr)
+
+      where "t '==<{' a '}>==>' t'" := (lts t a t')
+      and "t '--<{' a '}>-->' t'" := (Process.Semantics.step t a t').
+
+    Print lts.
+  End LTS.
+
+End System.
 
 
+(*************************************************************************)
+(**** Example ************************************************************)
+(*************************************************************************)
 
-Definition tmBool (b:bool) : tm := if true then TT else FF.
-Definition tmIBool (b:ibool) : tm := match b with | 0 => FF | 1 => TT | _ => TYPE_ERR end.
-
-Definition IsBool (v:var) : bool :=
-  match v with
-  | LOCKED => true
-  | SWAP => true
-  | _ => false
-  end.
-
-Definition IsIndex (v:var) : bool :=
-  match v with
-  | PREDECESSOR => true
-  | NEXT => true
-  | _ => false
-  end.
-
-Definition IsSome (o:option nat) : bool :=
-  match o with
-  | None => false
-  | Some _ => true
-  end.
-
-
-
-Definition tmIsNil (o:option nat) : tm := match o with | None => VAL TRU | _ => VAL FLS end.
-
-Definition tmIsTru (o:option nat) : tm := match o with | None => TYPE_ERR | Some b => tmIBool b end.
-
-Definition bind_predecessor (p:index) (s:state) : state :=
-  match s with
-  | (_pid, vars', _mem, _lock) =>
-    let vars'' := Build_vars (Some p) (acquire_locked vars') (release_next vars') (release_swap vars') in
-    (_pid, vars'', _mem, _lock)
-  end.
-
-Definition bind_locked (p:index) (s:state) : state :=
-  match s with
-  | (_pid, vars', _mem, _lock) =>
-    let vars'' := Build_vars (acquire_predecessor vars') (Some p) (release_next vars') (release_swap vars') in
-    (_pid, vars'', _mem, _lock)
-  end.
-
-Definition bind_next (p:index) (s:state) : state :=
-  match s with
-  | (_pid, vars', _mem, _lock) =>
-    let vars'' := Build_vars (acquire_predecessor vars') (acquire_locked vars') (Some p) (release_swap vars') in
-    (_pid, vars'', _mem, _lock)
-  end.
-
-Definition bind_swap (p:index) (s:state) : state :=
-  match s with
-  | (_pid, vars', _mem, _lock) =>
-    let vars'' := Build_vars (acquire_predecessor vars') (acquire_locked vars') (release_next vars') (Some p) in
-    (_pid, vars'', _mem, _lock)
-  end.
-
-
-(* initial *)
-Definition Initial_mem   (n:nat) : mem   := build_mem n.
-Definition Initial_lock          : lock  := (0, 0).
-Definition Initial_vars          : vars  := Build_vars None None None None.
-Definition Initial_state (n:nat) : state := (Nil, Initial_vars, Initial_mem n, Initial_lock).
-
-
-
-(* resulting term *)
-Definition tm_is_nil (v:val) (s:state) : tm :=
-  match v with
-  | VAR v' => if IsIndex v'
-              then tmIsNil (get_var v' s)
-              else TYPE_ERR
-  | TRU => FF
-  | FLS => FF
-  end.
-
-Definition tm_is_tru (v:val) (s:state) : tm :=
-  match v with
-  | VAR v' => if IsBool v'
-              then tmIsTru (get_var v' s)
-              else TYPE_ERR
-  | TRU => TT
-  | FLS => FF
-  end.
-
-
-
-(* substitution *)
-(* handle resulting terms *)
-
-
-Inductive action : Type := | SILENT : action | LABEL : act -> pid -> action.
-
-Definition step_state (a:act) (s:state) : state :=
-  match a with
-  (* CS Access *)
-  | NCS   => s
-  | ENTER => s
-  | LEAVE => s
-
-  (* Memory Access *)
-  | READ_NEXT    => bind_next   (get_mem_qnode_next   (Index (get_pid s)) s) s
-  | READ_LOCKED  => bind_locked (get_mem_qnode_locked (Index (get_pid s)) s) s
-
-  | WRITE_NEXT   pid_to_write next_pid  =>
-                    set_mem_qnode_next   (get_var pid_to_write s) (get_val next_pid  s) s
-
-  | WRITE_LOCKED pid_to_write is_locked =>
-                    set_mem_qnode_locked (get_var pid_to_write s) (get_val is_locked s) s
-
-  (* Lock Access *)
-  | FETCH_AND_STORE  => set_lock_i (Index (get_pid s)) (bind_predecessor (get_lock_i s) s)
-  | COMPARE_AND_SWAP => let s1 := set_lock_j (Index (get_pid s)) s in
-                        let s2 := bind_swap (index_eq (get_lock_i s1) (get_lock_j s1)) s1 in
-                        let s3 := set_lock_i 0 s2 in s3
-  end.
-
-
-Reserved Notation "t '--<{' a '}>-->' t'" (at level 40).
-
-Inductive step : (tm * state) -> action -> (tm * state) -> Prop :=
-
-  | ST_VAL_TRU : forall s, (VAL TRU, s) --<{SILENT}>--> (TT, s)
-  | ST_VAL_FLS : forall s, (VAL FLS, s) --<{SILENT}>--> (FF, s)
-
-  | ST_NOT_TT : forall s, (NOT TT, s) --<{SILENT}>--> (FF, s)
-  | ST_NOT_FF : forall s, (NOT FF, s) --<{SILENT}>--> (TT, s)
-
-  | ST_EQ_N : forall a b s, (EQ_N a b, s) --<{SILENT}>--> (tmBool (Nat.eqb a b), s)
-  | ST_EQ_B : forall a b s, (EQ_B a b, s) --<{SILENT}>--> (tmBool (eqb a b), s)
-
-  | ST_IS_NIL : forall v s,
-    (IS_NIL (VAL v), s) --<{SILENT}>--> (tm_is_nil v s, s)
-
-  | ST_IS_TRU : forall v s,
-    (IS_TRU (VAL v), s) --<{SILENT}>--> (tm_is_tru v s, s)
-
-  | ST_ACT : forall a t s, (ACT a t, s) --<{LABEL a (get_pid s)}>--> (t, step_state a s)
-
-  | ST_IF_TT : forall t1 t2 s, (<{ if TT then t1 else t2 }>, s) --<{SILENT}>--> (t1, s)
-  | ST_IF_FF : forall t1 t2 s, (<{ if FF then t1 else t2 }>, s) --<{SILENT}>--> (t2, s)
-
-  | ST_IF    : forall a c1 c2 t1 t2 s,
-    (c1, s) --<{a}>--> (c2, s) ->
-      (<{ if c1 then t1 else t2 }>, s) --<{SILENT}>--> (<{ if c2 then t1 else t2 }>, s)
-
-  | ST_SEQ_END : forall r s, (SEQ OK r, s) --<{SILENT}>--> (r, s)
-  | ST_SEQ     : forall a l1 l2 r s1 s2,
-    (l1, s1) --<{a}>--> (l2, s2) ->
-      (SEQ l1 r, s1) --<{a}>--> (SEQ l2 r, s2)
-
-  | ST_LOOP  : forall t s, (LOOP t, s) --<{SILENT}>--> (subst t LOOP_END false, s)
-  | ST_BREAK : forall l c s, (LOOP_OVER l (BREAK l) c, s) --<{SILENT}>--> (c, s)
-
-  | ST_LOOP_OVER : forall a l t1 t2 c s1 s2,
-    (LOOP t1, s1) --<{a}>--> (LOOP t2, s2) ->
-      (LOOP_OVER l t1 c, s1) --<{a}>--> (LOOP_OVER l t2 c, s2)
-
-  where "t '--<{' a '}>-->' t'" := (step t a t').
-
-
-Print step.
-
-Reserved Notation "t '==<{' a '}>==>' t'" (at level 40).
-
-Inductive sys : Type :=
-  | PRC : tm -> sys
-  | PAR : sys -> sys -> sys
-  .
-
-(* all tm must share the state, pass upwards to step. *)
-Inductive lts : sys * state -> action -> sys * state -> Prop :=
-
-  | LTS_PRC : forall a t1 t2 s1 s2,
-    (t1, s1) --<{a}>--> (t2, s2) ->
-      (PRC t1, s1) ==<{a}>==> (PRC t2, s2)
-
-  | LTS_TERM_L : forall a r s, (PAR (PRC OK) r, s) ==<{a}>==> (r, s)
-  | LTS_TERM_R : forall a l s, (PAR l (PRC OK), s) ==<{a}>==> (l, s)
-
-  | LTS_PAR_L : forall a l1 l2 r s1 s2,
-    (l1, s1) ==<{a}>==> (l2, s2) ->
-      (PAR l1 r, s1) ==<{a}>==> (PAR l2 r, s2)
-
-  | LTS_PAR_R : forall a l r1 r2 s1 s2,
-    (r1, s1) ==<{a}>==> (r2, s2) ->
-      (PAR l r1, s1) ==<{a}>==> (PAR l r2, s2)
-
-
-  where "t '==<{' a '}>==>' t'" := (lts t a t').
-
-Print lts.
-
-
-(*******************)
-(**** Example ******)
-(*******************)
+Import Process.
+Import Operation.
+Import Expr.
 
 Example Acquire : tm :=
-  ACT (WRITE_NEXT PID (VAR NIL)) (
-    ACT FETCH_AND_STORE (
-      IF (NOT (IS_NIL (VAL (VAR PREDECESSOR)))) (
-        ACT (WRITE_LOCKED PID TRU) (
-          ACT (WRITE_NEXT PREDECESSOR (VAR PID)) (
-            LOOP_OVER 0 (*L*) (
-              ACT READ_LOCKED (
-                IF (NOT (VAL (VAR LOCKED))) (
-                  BREAK 0 (*L*)
-                ) (OK)
-              )
-            ) (OK)
-          )
+  SEQ (ACT (WRITE_NEXT Vars.PID Val.NIL)) (
+    SEQ (ACT FETCH_AND_STORE) (
+      IF (NOT (EQ (VAR Vars.PREDECESSOR) NIL)) (
+        SEQ (ACT (WRITE_LOCKED Vars.PREDECESSOR (Val.PID))) (
+          LOOP_OVER 0 (
+            SEQ (ACT READ_LOCKED) (
+              IF (NOT (VAR Vars.LOCKED)) (BREAK 0) (OK)
+            )
+          ) (END)
         )
-      ) (OK)
+      ) (END)
     )
   ).
 
+
 Example Release : tm :=
-  ACT READ_NEXT (
-    IF (IS_NIL (VAL (VAR NEXT))) (
-      ACT COMPARE_AND_SWAP (
-        IF (NOT (IS_TRU (VAL (VAR SWAP)))) (
+  SEQ (ACT READ_NEXT) (
+    IF (EQ NIL (VAR Vars.NEXT)) (
+      SEQ (ACT COMPARE_AND_SWAP) (
+        IF (EQ FF (VAR Vars.SWAP)) (
           LOOP_OVER 0 (*L*) (
-            ACT READ_NEXT (
-              IF (NOT (IS_NIL (VAL (VAR NEXT)))) (
-                BREAK 0 (*L*)
-              ) (OK)
+            SEQ (ACT READ_NEXT) (
+              IF (NOT (EQ NIL (VAR Vars.NEXT))) (BREAK 0 (*L*)) (OK)
             )
-          ) (
-            ACT (WRITE_LOCKED NEXT TRU) (OK)
-          )
-        ) (OK)
+          ) (ACT (WRITE_LOCKED Vars.NEXT Val.TRU))
+        ) (END)
       )
-    ) (
-      ACT (WRITE_LOCKED NEXT FLS) (OK)
-    )
+    ) (ACT (WRITE_LOCKED Vars.NEXT Val.FLS))
   ).
+
 
 Example P : tm :=
   LOOP (
-    ACT NCS (
+    SEQ (ACT NCS) (
       SEQ Acquire (
-        ACT ENTER (
-          ACT LEAVE (
-            SEQ Release (OK)
+        SEQ (ACT ENTER) (
+          SEQ (ACT LEAVE) (
+            SEQ Release END
           )
         )
       )
     )
   ).
 
-Print P.
 
-Example config : tm * state := (P, Initial_state 1).
-Print config.
+Example p0 : tm * env := (P, (State.create 0, Resource.initial 0)).
+MeBi LTS Semantics.step p0.
 
-Example sys_config : sys * state := (PRC P, Initial_state 1).
-Print sys_config.
 
-MeBi LTS step config.
-MeBi LTS lts sys_config.
+(*******************************)
+(**** As part of a system ******)
+(*******************************)
+
+Definition process : Type := tm * State.local.
+Definition spawn (p:pid) (b:tm) : process := (b, State.create p).
+
+Fixpoint populate (n:nat) (b:tm) : list process :=
+  match n with
+  | 0 => []
+  | S m => app (populate m b) [spawn n b]
+  end.
+
+Definition system : Type := list process * Resource.resource.
+Definition create (n:nat) (b:tm) : system := (populate n b, Resource.initial n).
+
+Fixpoint load (ps:list process) : System.sys :=
+  match ps with
+  | [] => System.TERM
+  | h :: t =>
+    match h with
+    | (p, s) => System.PAR (System.PRC p s) (load t)
+    end
+  end.
+
+Definition composition : Type := System.sys * Resource.resource.
+Definition compose (s:system) : composition :=
+  match s with
+  | (ps, r) => (load ps, r)
+  end.
+
+Example ncs : composition := compose (create 5 P).
+MeBi LTS System.LTS.lts ncs.
